HOL --> MiniML translator builds again

examples/miniML/hol2miniml/std_preludeScript.sml
@@ -99,19 +99,17 @@ val res = translate GENLIST;
 val res = translate PAD_RIGHT;
 val res = translate PAD_LEFT;
 
-val _ = Parse.hide "MEM"
+val MEMBER_def = Define `
+  (MEMBER x [] = F) /\
+  (MEMBER x (y::ys) = (x = y) \/ MEMBER x ys)`;
 
-val MEM_def = Define `
-  (MEM x [] = F) /\
-  (MEM x (y::ys) = (x = y) \/ MEM x ys)`;
+val res = translate MEMBER_def;
 
-val res = translate MEM_def;
+val MEMBER_thm = prove(
+  ``!xs (x:'a). IS_EL x xs = MEMBER x xs``,
+  Induct THEN FULL_SIMP_TAC std_ss [MEM,MEMBER_def]);
 
-val MEM_thm = prove(
-  ``!xs (x:'a). IS_EL x xs = MEM x xs``,
-  Induct THEN FULL_SIMP_TAC std_ss [MEM,MEM_def]);
-
-val res = translate (ALL_DISTINCT |> REWRITE_RULE [MEM_thm]);
+val res = translate (ALL_DISTINCT |> REWRITE_RULE [MEMBER_thm]);
 val res = translate isPREFIX;
 val res = translate FRONT_DEF;
 val res = translate ZIP;
@@ -432,4 +430,3 @@ val LEAST_side_thm = prove(
   |> update_precondition;
 
 val _ = export_theory();
-
